Refactor types into single shared file to prevent anomalies with instantiating record types (#10)

proof/specs/XMSS_RFCAbs_RFCConc.ec
@@ -2,26 +2,42 @@ require import List.
 require import XMSS_PRF.
 require XMSS_Security_RFCAbs.
 
-import Types XMSS_Types Address BaseW Hash WOTS LTree XMSS_TreeHash.
-import Params OTSKeys.
+from Jasmin require import JModel.
+
+import Params Types Address BaseW Hash WOTS LTree XMSS_TreeHash OTSKeys.
 import ThreeNBytesBytes AuthPath.
 
 (* op prf_keygen : Params.nbytes -> Params.nbytes * Address.adrs -> Params.nbytes. *)
 (* op rand_hash : seed -> Address.adrs -> Params.nbytes -> Params.nbytes -> Params.nbytes. *)
 
 clone import XMSS_Security_RFCAbs as XMSSSecToAbs with
-  type XMSSRFCAbs.auth_path <- auth_path,
-  (* op XMSSRFCAbs.prf_keygen <- prf_keygen, *)
+  op XMSSRFCAbs.prf_keygen <- (fun (ss : nbytes) (psad : nbytes * adrs) =>
+                                prf_keygen (NBytes.val psad.`1 ++ NBytes.val (addr_to_bytes psad.`2)) ss),  (* prf_keygen, *)
   op XMSSRFCAbs.prf <- prf,
   op XMSSRFCAbs.f <- f,
-  (* op XMSSRFCAbs.rand_hash <- rand_hash, *)
+  op XMSSRFCAbs.rand_hash <- (fun (ps : seed) (ad : adrs) (l r : nbytes) => rand_hash l r ps ad),
   op XMSSRFCAbs.ltree <- ltree
-  proof *.
+proof *.
 
+import XMSSRFCAbs.
 
+module H_msg = {
+  proc o(mkm : threen_bytes * W8.t list) : nbytes = {
+    return H_msg mkm.`1 mkm.`2;
+  }
+}.
 
+equiv kg_eqv :
+  XMSS_RFC_Abs(H_msg).kg ~ XMSS_PRF.kg :
+  ={arg} ==> ={res}.
+proof. admitted.
 
+equiv sig_eqv :
+  XMSS_RFC_Abs(H_msg).sign ~ XMSS_PRF.sign :
+  ={arg} ==> ={res}.
+proof. admitted.
 
-
-
-
+equiv ver_eqv :
+  XMSS_RFC_Abs(H_msg).verify ~ XMSS_PRF.verify :
+  ={arg} ==> ={res}.
+proof. admitted.
